stdpp/zmap.v
@@ -20,72 +20,54 @@ Proof.
      cast_if_and3 (decide (x = y)) (decide (t1 = t2)) (decide (t1' = t2'))
   end); abstract congruence.
 Defined.
-Global Instance Zempty {A} : Empty (Zmap A) := ZMap None ∅ ∅.
-Global Instance Zlookup {A} : Lookup Z A (Zmap A) := λ i t,
+Global Instance Zmap_empty {A} : Empty (Zmap A) := ZMap None ∅ ∅.
+Global Instance Zmap_lookup {A} : Lookup Z A (Zmap A) := λ i t,
   match i with
   | Z0 => Zmap_0 t | Zpos p => Zmap_pos t !! p | Zneg p => Zmap_neg t !! p
   end.
-Global Instance Zpartial_alter {A} : PartialAlter Z A (Zmap A) := λ f i t,
+Global Instance Zmap_partial_alter {A} : PartialAlter Z A (Zmap A) := λ f i t,
   match i, t with
   | Z0, ZMap o t t' => ZMap (f o) t t'
-  | Zpos p, ZMap o t t' => ZMap o (partial_alter f p t) t'
-  | Zneg p, ZMap o t t' => ZMap o t (partial_alter f p t')
+  | Z.pos p, ZMap o t t' => ZMap o (partial_alter f p t) t'
+  | Z.neg p, ZMap o t t' => ZMap o t (partial_alter f p t')
   end.
-Global Instance Zto_list {A} : FinMapToList Z A (Zmap A) := λ t,
-  match t with
-  | ZMap o t t' => from_option (λ x, [(0,x)]) [] o ++
-     (prod_map Zpos id <$> map_to_list t) ++
-     (prod_map Zneg id <$> map_to_list t')
-  end.
-Global Instance Zomap: OMap Zmap := λ A B f t,
+Global Instance Zmap_fmap: FMap Zmap := λ A B f t,
+  match t with ZMap o t t' => ZMap (f <$> o) (f <$> t) (f <$> t') end.
+Global Instance Zmap_omap: OMap Zmap := λ A B f t,
   match t with ZMap o t t' => ZMap (o ≫= f) (omap f t) (omap f t') end.
-Global Instance Zmerge: Merge Zmap := λ A B C f t1 t2,
+Global Instance Zmap_merge: Merge Zmap := λ A B C f t1 t2,
   match t1, t2 with
   | ZMap o1 t1 t1', ZMap o2 t2 t2' =>
      ZMap (diag_None f o1 o2) (merge f t1 t2) (merge f t1' t2')
   end.
-Global Instance Zfmap: FMap Zmap := λ A B f t,
-  match t with ZMap o t t' => ZMap (f <$> o) (f <$> t) (f <$> t') end.
+Global Instance Zmap_fold {A} : MapFold Z A (Zmap A) := λ B f d t,
+  match t with
+  | ZMap mx t t' => map_fold (f ∘ Z.pos) (map_fold (f ∘ Z.neg)
+     match mx with Some x => f 0 x d | None => d end t') t
+  end.
 
-Global Instance: FinMap Z Zmap.
+Global Instance Zmap_map: FinMap Z Zmap.
 Proof.
   split.
   - intros ? [??] [??] H. f_equal.
     + apply (H 0).
-    + apply map_eq. intros i. apply (H (Zpos i)).
-    + apply map_eq. intros i. apply (H (Zneg i)).
+    + apply map_eq. intros i. apply (H (Z.pos i)).
+    + apply map_eq. intros i. apply (H (Z.neg i)).
   - by intros ? [].
   - intros ? f [] [|?|?]; simpl; [done| |]; apply lookup_partial_alter.
   - intros ? f [] [|?|?] [|?|?]; simpl; intuition congruence ||
       intros; apply lookup_partial_alter_ne; congruence.
   - intros ??? [??] []; simpl; [done| |]; apply lookup_fmap.
-  - intros ? [o t t']; unfold map_to_list; simpl.
-    assert (NoDup ((prod_map Z.pos id <$> map_to_list t) ++
-      (prod_map Z.neg id <$> map_to_list t'))).
-    { apply NoDup_app; split_and?.
-      - apply (NoDup_fmap_2 _), NoDup_map_to_list.
-      - intro. rewrite !elem_of_list_fmap. naive_solver.
-      - apply (NoDup_fmap_2 _), NoDup_map_to_list. }
-    destruct o; simpl; auto. constructor; auto.
-    rewrite elem_of_app, !elem_of_list_fmap. naive_solver.
-  - intros ? t i x. unfold map_to_list. split.
-    + destruct t as [[y|] t t']; simpl.
-      * rewrite elem_of_cons, elem_of_app, !elem_of_list_fmap.
-        intros [?|[[[??][??]]|[[??][??]]]]; simplify_eq/=; [done| |];
-          by apply elem_of_map_to_list.
-      * rewrite elem_of_app, !elem_of_list_fmap. intros [[[??][??]]|[[??][??]]];
-          simplify_eq/=; by apply elem_of_map_to_list.
-    + destruct t as [[y|] t t']; simpl.
-      * rewrite elem_of_cons, elem_of_app, !elem_of_list_fmap.
-        destruct i as [|i|i]; simpl; [intuition congruence| |].
-        { right; left. exists (i, x). by rewrite elem_of_map_to_list. }
-        right; right. exists (i, x). by rewrite elem_of_map_to_list.
-      * rewrite elem_of_app, !elem_of_list_fmap.
-        destruct i as [|i|i]; simpl; [done| |].
-        { left; exists (i, x). by rewrite elem_of_map_to_list. }
-        right; exists (i, x). by rewrite elem_of_map_to_list.
   - intros ?? f [??] [|?|?]; simpl; [done| |]; apply (lookup_omap f).
   - intros ??? f [??] [??] [|?|?]; simpl; [done| |]; apply (lookup_merge f).
+  - intros A B P f b Hemp Hinsert [mx t t'].
+    apply (map_fold_ind (λ r t, P r (ZMap mx t t'))); clear t.
+    { apply (map_fold_ind (λ r t', P r (ZMap mx ∅ t'))); clear t'.
+      { destruct mx as [x|]; [|done].
+        replace (ZMap (Some x) ∅ ∅) with (<[0:=x]> ∅ : Zmap _) by done.
+        by apply Hinsert. }
+      intros i x t' r ??. by apply (Hinsert (Z.neg i) x (ZMap mx ∅ t')). }
+    intros i x t r ??. by apply (Hinsert (Z.pos i) x (ZMap mx t t')).
 Qed.
 
 (** * Finite sets *)
